@prefix : <https://w3id.org/ride2rail/terms#> .
@prefix dc: <http://purl.org/dc/elements/1.1/> .
@prefix owl: <http://www.w3.org/2002/07/owl#> .
@prefix r2r: <https://w3id.org/ride2rail/terms#> .
@prefix rdf: <http://www.w3.org/1999/02/22-rdf-syntax-ns#> .
@prefix xml: <http://www.w3.org/XML/1998/namespace> .
@prefix xsd: <http://www.w3.org/2001/XMLSchema#> .
@prefix osdm: <https://w3id.org/mobility/osdm/core#> .
@prefix rdfs: <http://www.w3.org/2000/01/rdf-schema#> .
@prefix oasis: <http://www.dmi.unict.it/oasis.owl#> .
@prefix tmorg: <https://w3id.org/mobility/transmodel/organisations#> .
@base <https://w3id.org/ride2rail/terms#> .

<https://w3id.org/ride2rail/terms#> rdf:type owl:Ontology ;
                                     dc:creator "Mario Scrocca (Cefriel)" ;
                                     dc:description "Ontology describing the basic terms introduced by Ride2Rail for the modelling of smart contracts in the ledger module." ;
                                     dc:title "Ride2Rail Agreement Ledger Ontology" ;
                                     dc:license <https://creativecommons.org/licenses/by/4.0/> ;
                                     owl:versionInfo "1.0.0" .


#################################################################
#    Object Properties
#################################################################

###  https://w3id.org/ride2rail/terms#consumable
r2r:consumable rdf:type owl:ObjectProperty ;
               rdfs:domain r2r:InventoryAllocation ;
               rdfs:range r2r:Consumable ;
               rdfs:comment "Specify the type of Consumable associated with an InventoryAllocation." ;
               rdfs:label "consumable" .


###  https://w3id.org/ride2rail/terms#coversTravelEpisode
r2r:coversTravelEpisode rdf:type owl:ObjectProperty ;
                        rdfs:domain osdm:Offer ;
                        rdfs:range r2r:TravelEpisode ;
                        rdfs:comment "Specify a TravelEpisode covered by an Offer." ;
                        rdfs:label "covers travel episode" .


###  https://w3id.org/ride2rail/terms#hasOfferItem
r2r:hasOfferItem rdf:type owl:ObjectProperty ;
                 rdfs:domain osdm:Offer ;
                 rdfs:range r2r:OfferItem ;
                 rdfs:comment "An OfferItem composing an Offer." ;
                 rdfs:label "has offer item" .


###  https://w3id.org/ride2rail/terms#hasTransportationService
r2r:hasTransportationService rdf:type owl:ObjectProperty ;
                             rdfs:domain r2r:TravelEpisode ;
                             rdfs:range r2r:TransportationService ;
                             rdfs:comment "Associates a TravelEpisode with a TransportationService enabling it." ;
                             rdfs:label "has transportation service" .


###  https://w3id.org/ride2rail/terms#includesTravelEpisode
r2r:includesTravelEpisode rdf:type owl:ObjectProperty ;
                          rdfs:domain osdm:Trip ;
                          rdfs:range r2r:TravelEpisode ;
                          rdfs:comment "Associates a Trip with a TravelEpisode included in it." ;
                          rdfs:label "includes travel episode" .


###  https://w3id.org/ride2rail/terms#inventoryAllocation
r2r:inventoryAllocation rdf:type owl:ObjectProperty ;
                        rdfs:range r2r:InventoryAllocation ;
                        rdfs:comment "Associates an InventoryAllocation." ;
                        rdfs:label "inventory allocation" .


###  https://w3id.org/ride2rail/terms#issuedBy
r2r:issuedBy rdf:type owl:ObjectProperty ;
             rdfs:comment "Associates the subject with the Organisation issuing it." ;
             rdfs:label "issued by" .


###  https://w3id.org/ride2rail/terms#issuedTo
r2r:issuedTo rdf:type owl:ObjectProperty ;
             rdfs:comment "Associates the subject with the entity that is entitled to use the issued object." ;
             rdfs:label "issued to" .


###  https://w3id.org/ride2rail/terms#operatedBy
r2r:operatedBy rdf:type owl:ObjectProperty ;
               rdfs:domain r2r:TransportationService ;
               rdfs:range tmorg:Operator ;
               rdfs:comment "Associates a TransportationService with the Operator that performs it." ;
               rdfs:label "operated by" .

###  https://w3id.org/ride2rail/terms#hasRidesharingEvent
r2r:hasRidesharingEvent rdf:type owl:ObjectProperty ;
               rdfs:domain r2r:RidesharingBooking ;
               rdfs:range skos:Concept ;
               rdfs:comment "Associates a RidesharingBooking with a RidesharingBookingEvent." ;
               rdfs:label "has ridesharing event" .


#################################################################
#    Data properties
#################################################################

###  https://w3id.org/ride2rail/terms#discountPercentage
r2r:discountPercentage rdf:type owl:DatatypeProperty ;
                       rdfs:range xsd:integer ;
                       rdfs:comment "Specify the percentage of discount." ;
                       rdfs:label "discount percentage" .


###  https://w3id.org/ride2rail/terms#quantity
r2r:quantity rdf:type owl:DatatypeProperty ;
             rdfs:range xsd:integer ;
             rdfs:comment "Specify the quantity." ;
             rdfs:label "quantity" .


#################################################################
#    Classes
#################################################################


###  https://w3id.org/ride2rail/terms#RidesharingBooking
r2r:RidesharingBooking rdf:type owl:Class ;
               rdfs:subClassOf osdm:Booking ;
               rdfs:comment "A Booking associated with an OfferItem for a Ridesharing Leg." ;
               rdfs:label "Ridesharing Booking" .


###  https://w3id.org/ride2rail/terms#Consumable
r2r:Consumable rdf:type owl:Class ;
               rdfs:comment "A type of entity that can be listed in an InventoryAllocation and can be consumed performing a InventoryAllocation." ;
               rdfs:label "Consumable" .


###  https://w3id.org/ride2rail/terms#DiscountVoucher
r2r:DiscountVoucher rdf:type owl:Class ;
                    rdfs:subClassOf r2r:Voucher ,
                                    [ rdf:type owl:Restriction ;
                                      owl:onProperty r2r:discountPercentage ;
                                      owl:allValuesFrom xsd:integer
                                    ] ;
                    rdfs:comment "A voucher associated with a discount on the next purchase." ;
                    rdfs:label "Discount Voucher" .


###  https://w3id.org/ride2rail/terms#Driver
r2r:Driver rdf:type owl:Class ;
           rdfs:subClassOf tmorg:Operator ;
           rdfs:comment "A person offering a Ride for passengers covering a specific itinerary." ;
           rdfs:label "Driver" .


###  https://w3id.org/ride2rail/terms#IncentiveSmartContract
r2r:IncentiveSmartContract rdf:type owl:Class ;
                           rdfs:subClassOf oasis:SmartContract ;
                           rdfs:comment "Type of SmartContract defining incentives (providers, mechanisms, conditions)." ;
                           rdfs:label "Incentive Smart Contract" .


###  https://w3id.org/ride2rail/terms#InventoryAllocation
r2r:InventoryAllocation rdf:type owl:Class ;
                        rdfs:subClassOf [ rdf:type owl:Restriction ;
                                          owl:onProperty r2r:quantity ;
                                          owl:allValuesFrom xsd:integer
                                        ] ;
                        rdfs:comment "An InventoryAllocation describes a set of Consumables that can be reserved." ;
                        rdfs:label "Inventory Allocation" .


###  https://w3id.org/ride2rail/terms#InventoryReservation
r2r:InventoryReservation rdf:type owl:Class ;
                         rdfs:subClassOf osdm:Reservation ,
                                         [ rdf:type owl:Restriction ;
                                           owl:onProperty r2r:quantity ;
                                           owl:allValuesFrom xsd:integer
                                         ] ;
                         rdfs:comment "The reservation associated with an InventoryAllocation." ;
                         rdfs:label "Inventory Reservation" .


###  https://w3id.org/ride2rail/terms#OfferItem
r2r:OfferItem rdf:type owl:Class ;
              rdfs:subClassOf osdm:Offer ;
              rdfs:label "Offer Item" .


###  https://w3id.org/ride2rail/terms#Ride
r2r:Ride rdf:type owl:Class ;
         rdfs:subClassOf r2r:TransportationService ;
         rdfs:comment "A service offered by a Driver for passengers on a specific itinerary." ;
         rdfs:label "Ride" .


###  https://w3id.org/ride2rail/terms#RidesharingLeg
r2r:RidesharingLeg rdf:type owl:Class ;
                   rdfs:subClassOf r2r:TravelEpisode ;
                   rdfs:comment "A Travel Episode associated with a Ride." ;
                   rdfs:label "Ridesharing Leg" .


###  https://w3id.org/ride2rail/terms#SeatUpgradeVoucher
r2r:SeatUpgradeVoucher rdf:type owl:Class ;
                       rdfs:subClassOf r2r:Voucher ;
                       rdfs:comment "A Voucher associated with a seat upgrade for the next purchase." ;
                       rdfs:label "Seat Upgrade Voucher" .


###  https://w3id.org/ride2rail/terms#TransportationService
r2r:TransportationService rdf:type owl:Class ;
                          rdfs:comment "Service that provides transportation on a TravelEpisode." ;
                          rdfs:label "Transportation Service" .


###  https://w3id.org/ride2rail/terms#TravelEpisode
r2r:TravelEpisode rdf:type owl:Class ;
                  rdfs:comment "Part of a Trip, characterized by departure at a start point and arrival at the end point and operated with the same vehicle." ;
                  rdfs:label "Travel Episode" .


###  https://w3id.org/ride2rail/terms#Voucher
r2r:Voucher rdf:type owl:Class ;
            rdfs:comment "A bond for a redeemable good or benefit." ;
            rdfs:label "Voucher" .


#################################################################
#    Individuals
#################################################################


###  https://w3id.org/ride2rail/terms#Seats
r2r:Seats rdf:type owl:NamedIndividual ,
                   r2r:Consumable ;
          rdfs:comment "Type of Consumable describing seats in a vehicle." ;
          rdfs:label "Seats" .


###  https://w3id.org/ride2rail/terms#book
r2r:book rdf:type owl:NamedIndividual ,
                  oasis:Action ;
         rdfs:comment "Action representing a booking process." ;
         rdfs:label "book" .


###  https://w3id.org/ride2rail/terms#issue
r2r:issue rdf:type owl:NamedIndividual ,
                   oasis:Action ;
          rdfs:comment "Action representing an issuing process." ;
          rdfs:label "issue" .
